

# Derivations of Kriging Equations

Meredith Franklin

September 30, 2025

## 1 Lagrange Multipliers

Lagrange multipliers solve constrained extrema for  $f(x_1, \dots, x_n)$  subject to  $g(x_1, \dots, x_n) = 0$  when  $f, g$  are continuously differentiable and  $\nabla g \neq 0$ . At an extremum,  $\nabla f = -\lambda \nabla g$ .

For  $f(x, y) = x^2 + y^2$  and  $g(x, y) = x^2y - 16 = 0$ ,

$$L(x, y, \lambda) = x^2 + y^2 + \lambda(x^2y - 16).$$

First-order conditions (FOCs):

$$0 = \frac{\partial L}{\partial x} = 2x + 2\lambda xy = 2x(1 + \lambda y), \quad (1)$$

$$0 = \frac{\partial L}{\partial y} = 2y + \lambda x^2, \quad (2)$$

$$0 = \frac{\partial L}{\partial \lambda} = x^2y - 16. \quad (3)$$

From (1),  $x = 0$  or  $\lambda y = -1$ . The case  $x = 0$  contradicts (3), so  $\lambda = -1/y$ . Plugging into (2) gives  $2y - (x^2)/y = 0 \Rightarrow x^2 = 2y^2$ . With (3):  $x^2y = 16 \Rightarrow 2y^3 = 16 \Rightarrow y = 2$  and  $x = \pm 2\sqrt{2}$ . These two points are minima of  $f$  on  $x^2y = 16$ ; no maximum exists.

## 2 Ordinary Kriging (OK)

We want to predict  $Z(s_0)$  using a linear combination of observations:

$$\hat{Z}(s_0) = \sum_{i=1}^N w_i Z(s_i).$$

Unbiasedness condition

Because  $E[Z(s_i)] = \mu$  for all  $i$ , we have

$$E[\hat{Z}(s_0)] = \sum_{i=1}^N w_i E[Z(s_i)] = \mu \sum_{i=1}^N w_i.$$

For unbiasedness we require  $E[\hat{Z}(s_0)] = E[Z(s_0)] = \mu$ , which implies

$$\sum_{i=1}^N w_i = 1.$$

### Mean squared error (MSE)

The prediction error is

$$\hat{Z}(s_0) - Z(s_0) = \sum_{i=1}^N w_i Z(s_i) - Z(s_0).$$

The mean squared error (MSE) is

$$E[(\hat{Z}(s_0) - Z(s_0))^2] = \text{Var}(\hat{Z}(s_0) - Z(s_0)).$$

Expanding the variance term:

$$\text{Var}(\hat{Z}(s_0) - Z(s_0)) = \text{Var}\left(\sum_{i=1}^N w_i Z(s_i)\right) + \text{Var}[Z(s_0)] - 2 \text{Cov}\left(\sum_{i=1}^N w_i Z(s_i), Z(s_0)\right).$$

Each term separately:

$$\begin{aligned} \text{Var}\left(\sum_{i=1}^N w_i Z(s_i)\right) &= \sum_{i=1}^N \sum_{j=1}^N w_i w_j \text{Cov}[Z(s_i), Z(s_j)], \\ \text{Var}[Z(s_0)] &= C(0), \\ \text{Cov}\left(\sum_{i=1}^N w_i Z(s_i), Z(s_0)\right) &= \sum_{i=1}^N w_i \text{Cov}[Z(s_i), Z(s_0)]. \end{aligned}$$

So the MSE is

$$\text{MSE}(\mathbf{w}) = \mathbf{w}^\top \mathbf{C} \mathbf{w} + C(0) - 2\mathbf{w}^\top \mathbf{c},$$

where  $\mathbf{C} = (C_{ij})$  with  $C_{ij} = C(s_i - s_j)$  and  $\mathbf{c} = (C(s_i - s_0))$ .

### Constrained minimization

We minimize MSE subject to  $\mathbf{1}^\top \mathbf{w} = 1$  using the Lagrangian

$$L(\mathbf{w}, \lambda) = \mathbf{w}^\top \mathbf{C} \mathbf{w} + C(0) - 2\mathbf{w}^\top \mathbf{c} + 2\lambda(\mathbf{1}^\top \mathbf{w} - 1).$$

### First-order conditions (FOCs)

Differentiate with respect to  $\mathbf{w}$  and  $\lambda$ :

$$\begin{aligned} \frac{\partial L}{\partial \mathbf{w}} &= 2\mathbf{C} \mathbf{w} - 2\mathbf{c} + 2\lambda \mathbf{1} = \mathbf{0}, \\ \frac{\partial L}{\partial \lambda} &= 2(\mathbf{1}^\top \mathbf{w} - 1) = 0. \end{aligned}$$

Kriging system

Thus we obtain

$$\mathbf{C}\mathbf{w} + \lambda\mathbf{1} = \mathbf{c}, \quad \mathbf{1}^\top \mathbf{w} = 1.$$

Block matrix form:

$$\begin{bmatrix} \mathbf{C} & \mathbf{1} \\ \mathbf{1}^\top & 0 \end{bmatrix} \begin{bmatrix} \mathbf{w} \\ \lambda \end{bmatrix} = \begin{bmatrix} \mathbf{c} \\ 1 \end{bmatrix}.$$

Ordinary kriging variance

Plugging the optimal  $\mathbf{w}$  and  $\lambda$  back into the MSE yields

$$\sigma_{\text{OK}}^2 = C(0) - \mathbf{w}^\top \mathbf{c} - \lambda.$$

### 3 Universal Kriging (UK)

Suppose the mean is no longer constant but a linear combination of known functions:

$$Z(s) = \mu(s) + \varepsilon(s), \quad \mu(s) = \sum_{k=1}^p \beta_k f_k(s).$$

Predictor

We still predict as

$$\hat{Z}(s_0) = \sum_{i=1}^N w_i Z(s_i).$$

Unbiasedness constraints

We require  $E[\hat{Z}(s_0)] = E[Z(s_0)]$ . That is,

$$\sum_{i=1}^N w_i \mu(s_i) = \mu(s_0).$$

Since  $\mu(s) = \sum_k \beta_k f_k(s)$ , this implies

$$\sum_{i=1}^N w_i f_k(s_i) = f_k(s_0), \quad k = 1, \dots, p.$$

Matrix form: with  $F \in \mathbb{R}^{N \times p}$ ,  $F_{ik} = f_k(s_i)$  and  $\mathbf{f}_0 = (f_1(s_0), \dots, f_p(s_0))^\top$ , the constraints are

$$F^\top \mathbf{w} = \mathbf{f}_0.$$

### Mean squared error (MSE)

As before, the MSE is

$$\text{MSE}(\mathbf{w}) = \mathbf{w}^\top \mathbf{C} \mathbf{w} + C(0) - 2\mathbf{w}^\top \mathbf{c}.$$

### Constrained minimization

Now we minimize MSE subject to  $F^\top \mathbf{w} = \mathbf{f}_0$ . Introduce multipliers  $\boldsymbol{\lambda} = (\lambda_1, \dots, \lambda_p)^\top$  and write

$$L(\mathbf{w}, \boldsymbol{\lambda}) = \mathbf{w}^\top \mathbf{C} \mathbf{w} + C(0) - 2\mathbf{w}^\top \mathbf{c} + 2\boldsymbol{\lambda}^\top (F^\top \mathbf{w} - \mathbf{f}_0).$$

### First-order conditions (FOCs)

Differentiate:

$$\begin{aligned} \frac{\partial L}{\partial \mathbf{w}} &= 2\mathbf{C} \mathbf{w} - 2\mathbf{c} + 2F\boldsymbol{\lambda} = \mathbf{0}, \\ \frac{\partial L}{\partial \boldsymbol{\lambda}} &= 2(F^\top \mathbf{w} - \mathbf{f}_0) = \mathbf{0}. \end{aligned}$$

### Kriging system

This gives the UK system:

$$\begin{bmatrix} \mathbf{C} & F \\ F^\top & \mathbf{0} \end{bmatrix} \begin{bmatrix} \mathbf{w} \\ \boldsymbol{\lambda} \end{bmatrix} = \begin{bmatrix} \mathbf{c} \\ \mathbf{f}_0 \end{bmatrix}.$$

### Universal kriging variance

The minimized MSE is

$$\sigma_{\text{UK}}^2 = C(0) - \mathbf{w}^\top \mathbf{c} - \boldsymbol{\lambda}^\top \mathbf{f}_0.$$